renamed some symbols for clarity

Test/civl/inductive-sequentialization/2PC.bpl
@@ -18,22 +18,26 @@ function {:inline} pid (pid:int) : bool { 1 <= pid && pid <= n }
 function {:inline} pidLe (pid:int, k:int) : bool { 1 <= pid && pid <= k }
 function {:inline} pidGt (pid:int, k:int) : bool { k < pid && pid <= n }
 
-var {:layer 0,6} ReqCH:[int]int;           // Channel of the participants for request messages from the coordinator
-var {:layer 0,6} DecCH:[int][decision]int; // Channel of the participants for decision messages from the coordinator
-var {:layer 0,6} VoteCH:[vote]int;         // Channel of the coordinator for vote messages from the participants
-
-var {:layer 0,6} votes:[int]vote;          // Participant votes
-var {:layer 0,6} decisions:[int]decision;  // Coordinator and participant decisions
+// Channel of the participants for request messages from the coordinator
+var {:layer 0,6} RequestChannel:[int]int;
+// Channel of the participants for decision messages from the coordinator
+var {:layer 0,6} DecisionChannel:[int][decision]int;
+// Channel of the coordinator for vote messages from the participants
+var {:layer 0,6} VoteChannel:[vote]int;
+// Participant votes
+var {:layer 0,6} votes:[int]vote;
+// Coordinator and participant decisions
+var {:layer 0,6} decisions:[int]decision;
 
 ////////////////////////////////////////////////////////////////////////////////
 
-function {:inline} Init(pids:[int]bool, ReqCH:[int]int, VoteCH:[vote]int,
-  DecCH:[int][decision]int, decisions:[int]decision) : bool
+function {:inline} Init(pids:[int]bool, RequestChannel:[int]int, VoteChannel:[vote]int,
+  DecisionChannel:[int][decision]int, decisions:[int]decision) : bool
 {
   pids == MapConst(true) &&
-  ReqCH == (lambda i:int :: 0) &&
-  VoteCH == (lambda v:vote :: 0) &&
-  DecCH == (lambda i:int :: (lambda d:decision :: 0)) &&
+  RequestChannel == (lambda i:int :: 0) &&
+  VoteChannel == (lambda v:vote :: 0) &&
+  DecisionChannel == (lambda i:int :: (lambda d:decision :: 0)) &&
   decisions == (lambda i:int :: NONE())
 }
 
@@ -41,11 +45,11 @@ function {:inline} Init(pids:[int]bool, ReqCH:[int]int, VoteCH:[vote]int,
 
 procedure {:atomic}{:layer 6}
 MAIN5 ({:linear_in "pid"} pids:[int]bool)
-modifies ReqCH, VoteCH, votes, decisions;
+modifies RequestChannel, VoteChannel, votes, decisions;
 {
   var dec:decision;
-  assert Init(pids, ReqCH, VoteCH, DecCH, decisions);
-  havoc ReqCH, VoteCH, votes, decisions;
+  assert Init(pids, RequestChannel, VoteChannel, DecisionChannel, decisions);
+  havoc RequestChannel, VoteChannel, votes, decisions;
   if (*) { dec := COMMIT(); } else { dec := ABORT(); }
   assume dec == COMMIT() ==> (forall i:int :: pid(i) ==> votes[i] == YES());
   assume (forall i:int :: (i == 0 || pid(i)) ==> decisions[i] == dec);
@@ -55,37 +59,37 @@ procedure {:layer 5}
 {:creates "PARTICIPANT2"}
 {:IS_invariant}{:elim "PARTICIPANT2","PARTICIPANT2'"}
 INV4 ({:linear_in "pid"} pids:[int]bool)
-modifies ReqCH, VoteCH, DecCH, votes, decisions;
+modifies RequestChannel, VoteChannel, DecisionChannel, votes, decisions;
 {
   var {:pool "INV1"} k: int;
 
-  assert Init(pids, ReqCH, VoteCH, DecCH, decisions);
+  assert Init(pids, RequestChannel, VoteChannel, DecisionChannel, decisions);
 
   assume
     {:add_to_pool "INV1", k, k+1}
     {:add_to_pool "PARTICIPANT2", PARTICIPANT2(n)}
     0 <= k && k <= n;
-  havoc ReqCH, VoteCH, votes, decisions;
+  havoc RequestChannel, VoteChannel, votes, decisions;
   assume
     (decisions[0] == COMMIT() || decisions[0] == ABORT()) &&
     (decisions[0] == COMMIT() ==> (forall i:int :: pid(i) ==> votes[i] == YES())) &&
     (forall i:int :: pidLe(i,k) ==> decisions[i] == decisions[0]);
-  DecCH := (lambda i:int :: (lambda d:decision :: if pidGt(i, k) && d == decisions[0] then 1 else 0));
+  DecisionChannel := (lambda i:int :: (lambda d:decision :: if pidGt(i, k) && d == decisions[0] then 1 else 0));
   call create_asyncs((lambda {:pool "PARTICIPANT2"} pa:PARTICIPANT2 :: pidGt(pa->pid, k)));
   call set_choice(PARTICIPANT2(k+1));
 }
 
 procedure {:IS_abstraction}{:layer 5}
 PARTICIPANT2' ({:linear_in "pid"} pid:int)
-modifies DecCH, decisions;
+modifies DecisionChannel, decisions;
 {
   var d:decision;
   assert pid(pid);
-  assert DecCH[pid][NONE()] == 0;
-  assert DecCH[pid][COMMIT()] > 0 || DecCH[pid][ABORT()] > 0;
+  assert DecisionChannel[pid][NONE()] == 0;
+  assert DecisionChannel[pid][COMMIT()] > 0 || DecisionChannel[pid][ABORT()] > 0;
   if (*) { d := COMMIT(); } else { d := ABORT(); }
-  assume DecCH[pid][d] > 0;
-  DecCH[pid][d] := DecCH[pid][d] - 1;
+  assume DecisionChannel[pid][d] > 0;
+  DecisionChannel[pid][d] := DecisionChannel[pid][d] - 1;
   decisions[pid] := d;
 }
 
@@ -95,17 +99,17 @@ procedure {:atomic}{:layer 5}
 {:creates "PARTICIPANT2"}
 {:IS "MAIN5","INV4"}
 MAIN4 ({:linear_in "pid"} pids:[int]bool)
-modifies ReqCH, VoteCH, DecCH, votes, decisions;
+modifies RequestChannel, VoteChannel, DecisionChannel, votes, decisions;
 {
   var dec:decision;
-  assert Init(pids, ReqCH, VoteCH, DecCH, decisions);
+  assert Init(pids, RequestChannel, VoteChannel, DecisionChannel, decisions);
 
   assume {:add_to_pool "INV1", 0} true;
-  havoc ReqCH, VoteCH, votes;
+  havoc RequestChannel, VoteChannel, votes;
   if (*) { dec := COMMIT(); } else { dec := ABORT(); }
   assume dec == COMMIT() ==> (forall i:int :: pid(i) ==> votes[i] == YES());
   decisions[0] := dec;
-  DecCH := (lambda i:int :: (lambda d:decision :: if pid(i) && d == dec then 1 else 0));
+  DecisionChannel := (lambda i:int :: (lambda d:decision :: if pid(i) && d == dec then 1 else 0));
   call create_asyncs((lambda pa:PARTICIPANT2 :: pid(pa->pid)));
 }
 
@@ -113,18 +117,18 @@ procedure {:layer 4}
 {:creates "COORDINATOR2","PARTICIPANT2"}
 {:IS_invariant}{:elim "COORDINATOR2","COORDINATOR2'"}
 INV3 ({:linear_in "pid"} pids:[int]bool)
-modifies ReqCH, VoteCH, DecCH, votes, decisions;
+modifies RequestChannel, VoteChannel, DecisionChannel, votes, decisions;
 {
   var dec:decision;
-  assert Init(pids, ReqCH, VoteCH, DecCH, decisions);
+  assert Init(pids, RequestChannel, VoteChannel, DecisionChannel, decisions);
 
-  havoc ReqCH, VoteCH, votes;
+  havoc RequestChannel, VoteChannel, votes;
 
   if (*)
   {
-    assume VoteCH[YES()] >= 0 && VoteCH[NO()] >= 0;
-    assume VoteCH[YES()] + VoteCH[NO()] <= n;
-    assume VoteCH[YES()] == n ==> (forall i:int :: pid(i) ==> votes[i] == YES());
+    assume VoteChannel[YES()] >= 0 && VoteChannel[NO()] >= 0;
+    assume VoteChannel[YES()] + VoteChannel[NO()] <= n;
+    assume VoteChannel[YES()] == n ==> (forall i:int :: pid(i) ==> votes[i] == YES());
     call create_async(COORDINATOR2(0));
     call create_asyncs((lambda pa:PARTICIPANT2 :: pid(pa->pid)));
   }
@@ -133,21 +137,21 @@ modifies ReqCH, VoteCH, DecCH, votes, decisions;
     if (*) { dec := COMMIT(); } else { dec := ABORT(); }
     assume dec == COMMIT() ==> (forall i:int :: pid(i) ==> votes[i] == YES());
     decisions[0] := dec;
-    DecCH := (lambda i:int :: (lambda d:decision :: if pid(i) && d == dec then 1 else 0));
+    DecisionChannel := (lambda i:int :: (lambda d:decision :: if pid(i) && d == dec then 1 else 0));
     call create_asyncs((lambda pa:PARTICIPANT2 :: pid(pa->pid)));
   }
 }
 
 procedure {:IS_abstraction}{:layer 4}
 COORDINATOR2' ({:linear_in "pid"} pid:int)
-modifies VoteCH, DecCH, decisions;
+modifies VoteChannel, DecisionChannel, decisions;
 {
   var dec:decision;
   assert pid == 0;
 
   if (*)
   {
-    assume VoteCH[YES()] >= n;
+    assume VoteChannel[YES()] >= n;
     dec := COMMIT();
   }
   else
@@ -156,8 +160,8 @@ modifies VoteCH, DecCH, decisions;
   }
 
   decisions[pid] := dec;
-  havoc VoteCH;
-  DecCH := (lambda i:int :: (lambda d:decision :: if pid(i) && d == dec then DecCH[i][d] + 1 else DecCH[i][d]));
+  havoc VoteChannel;
+  DecisionChannel := (lambda i:int :: (lambda d:decision :: if pid(i) && d == dec then DecisionChannel[i][d] + 1 else DecisionChannel[i][d]));
 }
 
 ////////////////////////////////////////////////////////////////////////////////
@@ -166,13 +170,13 @@ procedure {:atomic}{:layer 4}
 {:creates "COORDINATOR2","PARTICIPANT2"}
 {:IS "MAIN4","INV3"}
 MAIN3 ({:linear_in "pid"} pids:[int]bool)
-modifies ReqCH, VoteCH, votes;
+modifies RequestChannel, VoteChannel, votes;
 {
-  assert Init(pids, ReqCH, VoteCH, DecCH, decisions);
-  havoc ReqCH, VoteCH, votes;
-  assume VoteCH[YES()] >= 0 && VoteCH[NO()] >= 0;
-  assume VoteCH[YES()] + VoteCH[NO()] <= n;
-  assume VoteCH[YES()] == n ==> (forall i:int :: pid(i) ==> votes[i] == YES());
+  assert Init(pids, RequestChannel, VoteChannel, DecisionChannel, decisions);
+  havoc RequestChannel, VoteChannel, votes;
+  assume VoteChannel[YES()] >= 0 && VoteChannel[NO()] >= 0;
+  assume VoteChannel[YES()] + VoteChannel[NO()] <= n;
+  assume VoteChannel[YES()] == n ==> (forall i:int :: pid(i) ==> votes[i] == YES());
   call create_async(COORDINATOR2(0));
   call create_asyncs((lambda pa:PARTICIPANT2 :: pid(pa->pid)));
 }
@@ -181,21 +185,21 @@ procedure {:layer 3}
 {:creates "COORDINATOR2","PARTICIPANT1","PARTICIPANT2"}
 {:IS_invariant}{:elim "PARTICIPANT1"}
 INV2 ({:linear_in "pid"} pids:[int]bool)
-modifies ReqCH, VoteCH, votes;
+modifies RequestChannel, VoteChannel, votes;
 {
   var {:pool "INV2"} k: int;
 
-  assert Init(pids, ReqCH, VoteCH, DecCH, decisions);
+  assert Init(pids, RequestChannel, VoteChannel, DecisionChannel, decisions);
 
-  havoc ReqCH, VoteCH, votes;
+  havoc RequestChannel, VoteChannel, votes;
   assume
     {:add_to_pool "INV2", k, k+1}
     {:add_to_pool "PARTICIPANT1", PARTICIPANT1(n)}
     0 <= k && k <= n;
-  assume (forall i:int :: pidGt(i,k) ==> ReqCH[i] == 1) &&
-    VoteCH[YES()] >= 0 && VoteCH[NO()] >= 0 &&
-    VoteCH[YES()] + VoteCH[NO()] <= k &&
-    (VoteCH[YES()] == k ==> (forall i:int :: pidLe(i,k) ==> votes[i] == YES()));
+  assume (forall i:int :: pidGt(i,k) ==> RequestChannel[i] == 1) &&
+    VoteChannel[YES()] >= 0 && VoteChannel[NO()] >= 0 &&
+    VoteChannel[YES()] + VoteChannel[NO()] <= k &&
+    (VoteChannel[YES()] == k ==> (forall i:int :: pidLe(i,k) ==> votes[i] == YES()));
   call create_async(COORDINATOR2(0));
   call create_asyncs((lambda pa:PARTICIPANT2 :: pidLe(pa->pid, k)));
   call create_asyncs((lambda {:pool "PARTICIPANT1"} pa:PARTICIPANT1 :: pidGt(pa->pid, k)));
@@ -208,12 +212,12 @@ procedure {:atomic}{:layer 3}
 {:creates "COORDINATOR2","PARTICIPANT1"}
 {:IS "MAIN3","INV2"}
 MAIN2 ({:linear_in "pid"} pids:[int]bool)
-modifies ReqCH;
+modifies RequestChannel;
 {
-  assert Init(pids, ReqCH, VoteCH, DecCH, decisions);
+  assert Init(pids, RequestChannel, VoteChannel, DecisionChannel, decisions);
 
   assume {:add_to_pool "INV2", 0} true;
-  ReqCH := (lambda i:int :: if pid(i) then 1 else 0);
+  RequestChannel := (lambda i:int :: if pid(i) then 1 else 0);
   call create_async(COORDINATOR2(0));
   call create_asyncs((lambda pa:PARTICIPANT1 :: pid(pa->pid)));
 }
@@ -222,9 +226,9 @@ procedure {:layer 2}
 {:creates "COORDINATOR1","COORDINATOR2","PARTICIPANT1"}
 {:IS_invariant}{:elim "COORDINATOR1"}
 INV1 ({:linear_in "pid"} pids:[int]bool)
-modifies ReqCH;
+modifies RequestChannel;
 {
-  assert Init(pids, ReqCH, VoteCH, DecCH, decisions);
+  assert Init(pids, RequestChannel, VoteChannel, DecisionChannel, decisions);
   if (*)
   {
     call create_async(COORDINATOR1(0));
@@ -232,7 +236,7 @@ modifies ReqCH;
   }
   else
   {
-    ReqCH := (lambda i:int :: if pid(i) then 1 else 0);
+    RequestChannel := (lambda i:int :: if pid(i) then 1 else 0);
     call create_async(COORDINATOR2(0));
     call create_asyncs((lambda pa:PARTICIPANT1 :: pid(pa->pid)));
   }
@@ -245,7 +249,7 @@ procedure {:atomic}{:layer 2}
 {:IS "MAIN2","INV1"}
 MAIN1 ({:linear_in "pid"} pids:[int]bool)
 {
-  assert Init(pids, ReqCH, VoteCH, DecCH, decisions);
+  assert Init(pids, RequestChannel, VoteChannel, DecisionChannel, decisions);
   call create_async(COORDINATOR1(0));
   call create_asyncs((lambda pa:PARTICIPANT1 :: pid(pa->pid)));
 }
@@ -254,18 +258,18 @@ procedure {:atomic}{:layer 2,3}
 {:pending_async}
 {:creates "PARTICIPANT2"}
 PARTICIPANT1 ({:linear_in "pid"} pid:int)
-modifies ReqCH, VoteCH, votes;
+modifies RequestChannel, VoteChannel, votes;
 {
   var v:vote;
   assert pid(pid);
 
   if (*)
   {
-    assume ReqCH[pid] > 0;
-    ReqCH[pid] := ReqCH[pid] - 1;
+    assume RequestChannel[pid] > 0;
+    RequestChannel[pid] := RequestChannel[pid] - 1;
     if (*) { v := YES(); } else { v := NO(); }
     votes[pid] := v;
-    VoteCH[v] := VoteCH[v] + 1;
+    VoteChannel[v] := VoteChannel[v] + 1;
   }
 
   call create_async(PARTICIPANT2(pid));
@@ -274,14 +278,14 @@ modifies ReqCH, VoteCH, votes;
 procedure {:atomic}{:layer 2,5}
 {:pending_async}
 PARTICIPANT2 ({:linear_in "pid"} pid:int)
-modifies DecCH, decisions;
+modifies DecisionChannel, decisions;
 {
   var d:decision;
   assert pid(pid);
-  assert DecCH[pid][NONE()] == 0;
+  assert DecisionChannel[pid][NONE()] == 0;
   if (*) { d := COMMIT(); } else { d := ABORT(); }
-  assume DecCH[pid][d] > 0;
-  DecCH[pid][d] := DecCH[pid][d] - 1;
+  assume DecisionChannel[pid][d] > 0;
+  DecisionChannel[pid][d] := DecisionChannel[pid][d] - 1;
   decisions[pid] := d;
 }
 
@@ -289,45 +293,45 @@ procedure {:left}{:layer 2}
 {:pending_async}
 {:creates "COORDINATOR2"}
 COORDINATOR1 ({:linear_in "pid"} pid:int)
-modifies ReqCH;
+modifies RequestChannel;
 {
   assert pid == 0;
-  ReqCH := (lambda i:int :: if pid(i) then ReqCH[i] + 1 else ReqCH[i]);
+  RequestChannel := (lambda i:int :: if pid(i) then RequestChannel[i] + 1 else RequestChannel[i]);
   call create_async(COORDINATOR2(0));
 }
 
 procedure {:atomic}{:layer 2,4}
 {:pending_async}
 COORDINATOR2 ({:linear_in "pid"} pid:int)
-modifies VoteCH, DecCH, decisions;
+modifies VoteChannel, DecisionChannel, decisions;
 {
   var dec:decision;
   assert pid == 0;
 
   if (*)
   {
-    assume VoteCH[YES()] >= n;
-    VoteCH[YES()] := VoteCH[YES()] - n;
+    assume VoteChannel[YES()] >= n;
+    VoteChannel[YES()] := VoteChannel[YES()] - n;
     dec := COMMIT();
   }
   else
   {
-    assume VoteCH[NO()] > 0;
-    havoc VoteCH;
-    assume VoteCH[NO()] == old(VoteCH)[NO()] - 1;
-    assume 0 <= VoteCH[YES()] && VoteCH[YES()] <= old(VoteCH)[YES()];
+    assume VoteChannel[NO()] > 0;
+    havoc VoteChannel;
+    assume VoteChannel[NO()] == old(VoteChannel)[NO()] - 1;
+    assume 0 <= VoteChannel[YES()] && VoteChannel[YES()] <= old(VoteChannel)[YES()];
     dec := ABORT();
   }
 
   decisions[pid] := dec;
-  DecCH := (lambda i:int :: (lambda d:decision :: if pid(i) && d == dec then DecCH[i][d] + 1 else DecCH[i][d]));
+  DecisionChannel := (lambda i:int :: (lambda d:decision :: if pid(i) && d == dec then DecisionChannel[i][d] + 1 else DecisionChannel[i][d]));
 }
 
 ////////////////////////////////////////////////////////////////////////////////
 
 procedure {:yields}{:layer 1}{:refines "MAIN1"}
 main ({:linear_in "pid"} pids:[int]bool)
-requires {:layer 1} Init(pids, ReqCH, VoteCH, DecCH, decisions);
+requires {:layer 1} Init(pids, RequestChannel, VoteChannel, DecisionChannel, decisions);
 {
   var i:int;
   var {:pending_async}{:layer 1} Coordinator1_PAs:[COORDINATOR1]int;
@@ -374,26 +378,26 @@ requires {:layer 1} pid(pid);
 {
   var d:decision;
 
-  call d := receive_dec(pid);
+  call d := receive_decision(pid);
   call set_decision(pid, d);
 }
 
 procedure {:yields}{:layer 1}{:refines "COORDINATOR1"}
 coordinator1 ({:linear_in "pid"} pid:int)
 requires {:layer 1} pid == 0;
-requires {:layer 1} (forall vv:vote :: VoteCH[vv] >= 0);
+requires {:layer 1} (forall vv:vote :: VoteChannel[vv] >= 0);
 {
   var i:int;
-  var {:layer 1} old_ReqCH:[int]int;
+  var {:layer 1} old_RequestChannel:[int]int;
 
-  call old_ReqCH := Snapshot_ReqCH();
+  call old_RequestChannel := Snapshot_RequestChannel();
   i := 1;
   while (i <= n)
   invariant {:layer 1}{:cooperates} true;
   invariant {:layer 1} 1 <= i && i <= n+1;
-  invariant {:layer 1} ReqCH == (lambda ii:int :: if pid(ii) && ii < i then old_ReqCH[ii] + 1 else old_ReqCH[ii]);
+  invariant {:layer 1} RequestChannel == (lambda ii:int :: if pid(ii) && ii < i then old_RequestChannel[ii] + 1 else old_RequestChannel[ii]);
   {
-    call send_req(i);
+    call send_request(i);
     i := i + 1;
   }
   async call coordinator2(pid);
@@ -402,23 +406,23 @@ requires {:layer 1} (forall vv:vote :: VoteCH[vv] >= 0);
 procedure {:yields}{:layer 1}{:refines "COORDINATOR2"}
 coordinator2 ({:linear_in "pid"} pid:int)
 requires {:layer 1} pid == 0;
-requires {:layer 1} (forall vv:vote :: VoteCH[vv] >= 0);
+requires {:layer 1} (forall vv:vote :: VoteChannel[vv] >= 0);
 {
   var d:decision;
   var v:vote;
   var i:int;
-  var {:layer 1} old_VoteCH:[vote]int;
-  var {:layer 1} old_DecCH:[int][decision]int;
+  var {:layer 1} old_VoteChannel:[vote]int;
+  var {:layer 1} old_DecisionChannel:[int][decision]int;
 
-  call old_VoteCH := Snapshot_VoteCH();
-  call old_DecCH := Snapshot_DecCH();
+  call old_VoteChannel := Snapshot_VoteChannel();
+  call old_DecisionChannel := Snapshot_DecisionChannel();
   i := 0;
   d := COMMIT();
   while (i < n)
   invariant {:layer 1} 0 <= i && i <= n;
-  invariant {:layer 1} VoteCH[YES()] == old_VoteCH[YES()] - i;
-  invariant {:layer 1} old_VoteCH[YES()] - i >= 0;
-  invariant {:layer 1} VoteCH[NO()] == old_VoteCH[NO()];
+  invariant {:layer 1} VoteChannel[YES()] == old_VoteChannel[YES()] - i;
+  invariant {:layer 1} old_VoteChannel[YES()] - i >= 0;
+  invariant {:layer 1} VoteChannel[NO()] == old_VoteChannel[NO()];
   {
     call v := receive_vote();
     if (v == NO())
@@ -433,26 +437,26 @@ requires {:layer 1} (forall vv:vote :: VoteCH[vv] >= 0);
   while (i <= n)
   invariant {:layer 1}{:cooperates} true;
   invariant {:layer 1} 1 <= i && i <= n+1;
-  invariant {:layer 1} DecCH == (lambda ii:int :: (lambda dd:decision :: if pid(ii) && ii < i && dd == d then old_DecCH[ii][dd] + 1 else old_DecCH[ii][dd]));
+  invariant {:layer 1} DecisionChannel == (lambda ii:int :: (lambda dd:decision :: if pid(ii) && ii < i && dd == d then old_DecisionChannel[ii][dd] + 1 else old_DecisionChannel[ii][dd]));
   {
-    call send_dec(i, d);
+    call send_decision(i, d);
     i := i + 1;
   }
 }
 
-procedure {:intro}{:layer 1} Snapshot_ReqCH() returns (snapshot:[int]int)
+procedure {:intro}{:layer 1} Snapshot_RequestChannel() returns (snapshot:[int]int)
 {
-  snapshot := ReqCH;
+  snapshot := RequestChannel;
 }
 
-procedure {:intro}{:layer 1} Snapshot_VoteCH() returns (snapshot:[vote]int)
+procedure {:intro}{:layer 1} Snapshot_VoteChannel() returns (snapshot:[vote]int)
 {
-  snapshot := VoteCH;
+  snapshot := VoteChannel;
 }
 
-procedure {:intro}{:layer 1} Snapshot_DecCH() returns (snapshot:[int][decision]int)
+procedure {:intro}{:layer 1} Snapshot_DecisionChannel() returns (snapshot:[int][decision]int)
 {
-  snapshot := DecCH;
+  snapshot := DecisionChannel;
 }
 
 ////////////////////////////////////////////////////////////////////////////////
@@ -469,53 +473,53 @@ modifies decisions;
   decisions[pid] := d;
 }
 
-procedure {:left}{:layer 1} SEND_REQ(pid:int)
-modifies ReqCH;
+procedure {:left}{:layer 1} SEND_REQUEST(pid:int)
+modifies RequestChannel;
 {
-  ReqCH[pid] := ReqCH[pid] + 1;
+  RequestChannel[pid] := RequestChannel[pid] + 1;
 }
 
 procedure {:right}{:layer 1} RECEIVE_REQ(pid:int)
-modifies ReqCH;
+modifies RequestChannel;
 {
-  assume ReqCH[pid] > 0;
-  ReqCH[pid] := ReqCH[pid] - 1;
+  assume RequestChannel[pid] > 0;
+  RequestChannel[pid] := RequestChannel[pid] - 1;
 }
 
 procedure {:left}{:layer 1} SEND_VOTE(v:vote)
-modifies VoteCH;
+modifies VoteChannel;
 {
-  VoteCH[v] := VoteCH[v] + 1;
+  VoteChannel[v] := VoteChannel[v] + 1;
 }
 
 procedure {:right}{:layer 1} RECEIVE_VOTE() returns (v:vote)
-modifies VoteCH;
+modifies VoteChannel;
 {
-  assume VoteCH[v] > 0;
-  VoteCH[v] := VoteCH[v] - 1;
+  assume VoteChannel[v] > 0;
+  VoteChannel[v] := VoteChannel[v] - 1;
 }
 
-procedure {:left}{:layer 1} SEND_DEC(pid:int, d:decision)
-modifies DecCH;
+procedure {:left}{:layer 1} SEND_DECISION(pid:int, d:decision)
+modifies DecisionChannel;
 {
-  DecCH[pid][d] := DecCH[pid][d] + 1;
+  DecisionChannel[pid][d] := DecisionChannel[pid][d] + 1;
 }
 
-procedure {:right}{:layer 1} RECEIVE_DEC(pid:int) returns (d:decision)
-modifies DecCH;
+procedure {:right}{:layer 1} RECEIVE_DECISION(pid:int) returns (d:decision)
+modifies DecisionChannel;
 {
-  assume DecCH[pid][d] > 0;
-  DecCH[pid][d] := DecCH[pid][d] - 1;
+  assume DecisionChannel[pid][d] > 0;
+  DecisionChannel[pid][d] := DecisionChannel[pid][d] - 1;
 }
 
 procedure {:yields}{:layer 0}{:refines "SET_VOTE"} set_vote({:linear "pid"} pid:int, v:vote);
 procedure {:yields}{:layer 0}{:refines "SET_DECISION"} set_decision({:linear "pid"} pid:int, d:decision);
-procedure {:yields}{:layer 0}{:refines "SEND_REQ"} send_req(pid:int);
+procedure {:yields}{:layer 0}{:refines "SEND_REQUEST"} send_request(pid:int);
 procedure {:yields}{:layer 0}{:refines "RECEIVE_REQ"} receive_req(pid:int);
 procedure {:yields}{:layer 0}{:refines "SEND_VOTE"} send_vote(v:vote);
 procedure {:yields}{:layer 0}{:refines "RECEIVE_VOTE"} receive_vote() returns (v:vote);
-procedure {:yields}{:layer 0}{:refines "SEND_DEC"} send_dec(pid:int, d:decision);
-procedure {:yields}{:layer 0}{:refines "RECEIVE_DEC"} receive_dec(pid:int) returns (d:decision);
+procedure {:yields}{:layer 0}{:refines "SEND_DECISION"} send_decision(pid:int, d:decision);
+procedure {:yields}{:layer 0}{:refines "RECEIVE_DECISION"} receive_decision(pid:int) returns (d:decision);
 
 procedure {:both}{:layer 1}
 LINEAR_TRANSFER(i:int, {:linear_in "pid"} pids:[int]bool)
